meminj decomposed

cklr/Inject.v
@@ -537,13 +537,7 @@ Proof.
     + cbn. rstep; auto.
 Qed.
 
-(*Lemma decompose_meminj:
-  forall f1 f2 f',
-    inject_incr (compose_meminj f1 f2) f' ->
-    exists f1' f2',
-      compose_meminj f1' f2' =  *)
-
-
+(*test *)
 Definition meminj_incr_sep (f1 f2 f3 : meminj) : Prop :=
   forall b, f2 b =
     match f1 b with
@@ -560,144 +554,151 @@ Proof.
   apply H in Heqo. eauto. congruence.
   intros. rewrite H0 in H1. congruence.
 Qed.
-(*
-Theorem meminj_incr_codomain:
-  forall f1 f2, inject_incr f1 f2 ->
-  exists list,( forall b, (f1 b = None /\ f2 b <> None) <-> In b list).
-Proof.
-  intros.
-*)
-Lemma inject_compose_inv:
+
+(*Lemma inject_compose_inv:
   forall (f f': meminj) (m1 m2 m3: mem),
     Mem.inject (compose_meminj f f') m1 m3 ->
     exists m2, Mem.inject f m1 m2 /\
           Mem.inject f' m2 m3.
 Proof. Abort.
+*)
 
 Definition meminj_add (f:meminj) b1 r:=
   fun b => if (eq_block b b1) then Some r else f b.
 
-Definition new_mapped_block (f10 f':meminj) (b:block) : bool :=
-  match f10 b, f' b with
-    |None, Some _ => true
-    | _,_ => false
+Lemma meminj_add_new: forall f a b,
+    meminj_add f a b a = Some b.
+Proof.
+  intros. unfold meminj_add. rewrite pred_dec_true; auto. Qed.
+
+Fixpoint update_meminj12 (s1 s1' : list block) (f10 f02 f': meminj) (smid: sup) :=
+  match s1' with
+    |nil => (f10,f02,smid)
+    |hd::tl => if (Mem.sup_dec hd s1) then update_meminj12 s1 tl f10 f02 f' smid else
+                (
+              let b0 := fresh_block smid in
+              match f' hd with
+                |Some r =>
+                update_meminj12 (hd::s1) tl (meminj_add f10 hd (b0,0) )
+                                   (meminj_add f02 (fresh_block smid) r)
+                                f' (sup_incr smid)
+                |_ =>
+                update_meminj12 s1 tl f10 f02 f' smid
+              end)
   end.
 
-Fixpoint update_meminj1 (support1 : list block) (f10 f': meminj) (sup1: sup) :=
-  match support1 with
-    |nil => f10
-    |hd::tl => let b0 := fresh_block sup1 in
-                if (new_mapped_block f10 f' hd) then
-                update_meminj1 tl (meminj_add f10 hd (b0,0)) f'
-                               (sup_incr sup1) else 
-                update_meminj1 tl f10 f' sup1
-  end.
-
-Fixpoint update_meminj12 (support1 : list block) (f10 f02 f': meminj) (sup1: sup) :=
-  match support1 with
-    |nil => (f10,f02)
-    |hd::tl => let b0 := fresh_block sup1 in
-              match f10 hd, f' hd with
-                |None, Some r =>
-                update_meminj12 tl (meminj_add f10 hd (b0,0) )
-                                   (meminj_add f02 (fresh_block sup1) r)
-                                f' (sup_incr sup1)
-                |_,_ =>
-                update_meminj12 tl f10 f02 f' sup1
-              end
-  end.
-
-Lemma update_properties: forall l1 f10 f02 s f10' f02' f',
-    update_meminj12 l1 f10 f02 f' s = (f10',f02') ->
+Lemma update_properties: forall s1' s1 f10 f02 s s' f10' f02' f',
+    update_meminj12 s1 s1' f10 f02 f' s = (f10',f02',s') ->
     (forall b, ~sup_In b s -> f02 b = None) ->
+    (forall b, ~sup_In b s1 -> f10 b = None) ->
     (*Mem.inject f10 m1 m0 ->
     Mem.inject f02 m0 m2 ->
     Mem.inject f' m1' m2' ->
     inject_incr (compose_meminj f10 f02) f' ->
     Mem.sup_include (Mem.support m1) (Mem.support m1') ->
     Mem.sup_include (Mem.support m2) (Mem.support m2') -> *)
-    inject_incr f10 f10' /\ inject_incr f02 f02'
+    inject_incr f10 f10' /\ inject_incr f02 f02' /\ Mem.sup_include s s'
     /\ (forall (b1 b0 : block) (delta : Z),
         f10 b1 = None -> f10' b1 = Some (b0, delta) -> (exists b2 ofs2, f' b1 = Some (b2,ofs2)) /\ ~ sup_In b0 s)
     /\ (forall (b0 b2 : block) (delta : Z),
-        f02 b0 = None -> f02' b0 = Some (b2, delta) -> ~ sup_In b0 s /\ (exists b1, f10 b1 = None /\ f' b1 = Some (b2,delta)))
-(*    /\ (forall b1 b2 ofs, f' b1 = Some (b2, ofs) -> exists b0 ofs0, f10' b1 = Some (b0,ofs0) /\ f02' b0 = Some (b2,ofs)) *). 
+        f02 b0 = None -> f02' b0 = Some (b2, delta) -> ~ sup_In b0 s /\ (exists b1, f10 b1 = None /\ f' b1 = Some (b2,delta))).
 Proof.
-  induction l1; intros; inv H.
+  induction s1'; intros; inv H.
   - split. eauto. split. eauto. split. congruence.
     split; congruence.
-  - destruct (f10 a) eqn:?.
-    + eauto.
-    + destruct (f' a) eqn:?.
-      (*update case*)
-    apply IHl1 in H2.
+  - destruct Mem.sup_dec in H3. eauto.
+    destruct (f' a) eqn:?.
+    (*update case*)
+    apply IHs1' in H3.
     assert (inject_incr f10 (meminj_add f10 a (fresh_block s,0))).
     unfold meminj_add.
-    intro. intros.  destruct (eq_block b a). congruence. auto.
+    intro. intros.  destruct (eq_block b a). apply H1 in n. congruence. auto.
     assert (inject_incr f02 (meminj_add f02 (fresh_block s) p)).
     intro. unfold meminj_add. intros.
     destruct eq_block. exploit H0. apply freshness. intro. congruence.
-    eauto. destruct H2 as (incr1& incr2 & sep1 & sep2).
+    eauto. destruct H3 as (incr1& incr2 & sinc  & sep1 & sep2).
     (*incr1*)
     split. eapply inject_incr_trans; eauto.
     (*incr2*)
     split. eapply inject_incr_trans; eauto.
+    (*sinc*)
+    split. eapply Mem.sup_include_trans; eauto.
     (*sep1*)
     split.
     intros. destruct (meminj_add f10 a (fresh_block s,0) b1) eqn: Hab.
     unfold meminj_add in Hab. destruct eq_block in Hab. subst. inv Hab.
     assert (meminj_add f10 a (fresh_block s,0) a = Some (fresh_block s,0)).
     unfold meminj_add. rewrite pred_dec_true. auto. auto.
-    apply incr1 in H4.
-    rewrite H3 in H4. inv H4.
+    apply incr1 in H5.
+    rewrite H4 in H5. inv H5.
     assert (meminj_add f02 (fresh_block s) p (fresh_block s) = Some p).
     unfold meminj_add. rewrite pred_dec_true; eauto. destruct p.
-    apply incr2 in H4. split.
+    apply incr2 in H5. split.
     exists b,z.  congruence.
     apply freshness.
     congruence.
-    exploit sep1; eauto. intros. inv H4. split. auto.
-    intro. apply H6. apply Mem.sup_incr_in2. eauto.
+    exploit sep1; eauto. intros. inv H5. split. auto.
+    intro. apply H7. apply Mem.sup_incr_in2. eauto.
     (*sep2*)
     intros. destruct p. destruct (meminj_add f02 (fresh_block s) (b,z) b0) eqn: Hab.
     unfold meminj_add in Hab. destruct eq_block in Hab. subst. inv Hab.
     assert (meminj_add f02 (fresh_block s) (b,z) (fresh_block s) = Some (b,z)).
     unfold meminj_add. rewrite pred_dec_true. auto. auto.
-    apply incr2 in H4.
-    rewrite H3 in H4. inv H4.
+    apply incr2 in H5.
+    rewrite H4 in H5. inv H5.
     split. apply freshness.
-    exists a. split;  congruence.
+    exists a. split. apply H1. auto.  congruence.
     congruence.
-    exploit sep2; eauto. intros. inv H4. split.
-    intro. apply H5. apply Mem.sup_incr_in2. eauto.
-    destruct H6 as (b1 & A & B).
+    exploit sep2; eauto. intros. inv H5. split.
+    intro. apply H6. apply Mem.sup_incr_in2. eauto.
+    destruct H7 as (b1 & A & B).
     exists b1. split.  unfold meminj_add in A. destruct eq_block in A. congruence. auto.
     auto.
     (*condition1*)
-    intros.
     intros. unfold meminj_add. destruct eq_block. subst.
     elim H. apply Mem.sup_incr_in1. apply H0. intro. apply H.
     apply Mem.sup_incr_in2. eauto.
+    (*condition2*)
+    intros. unfold meminj_add. destruct eq_block. subst.
+    elim H. left. auto. apply H1. intro. apply H. right. auto.
     eauto.
 Qed.
 
-Lemma update_properties2: forall l1 f10 f02 s f10' f02' f',
-    update_meminj12 l1 f10 f02 f' s = (f10',f02') ->
-    inject_incr (compose_meminj f10 f02) f' ->
-    (forall b, ~ sup_In b l1 -> f' b = None) ->
-    (*Mem.inject f10 m1 m0 ->
-    Mem.inject f02 m0 m2 ->
-    Mem.inject f' m1' m2' ->
-    inject_incr (compose_meminj f10 f02) f' ->
-    Mem.sup_include (Mem.support m1) (Mem.support m1') ->
-    Mem.sup_include (Mem.support m2) (Mem.support m2') -> *)
-    (forall b1 b2 ofs, f' b1 = Some (b2, ofs) -> exists b0 ofs0, f10' b1 = Some (b0,ofs0) /\ f02' b0 = Some (b2,ofs)). 
+Lemma update_properties2: forall s1' s1 f10 f02 s s' f10' f02' f' b b' ofs,
+    update_meminj12 s1 s1' f10 f02 f' s = (f10',f02',s') ->
+   (forall b, ~sup_In b s -> f02 b = None) ->
+    (forall b, ~sup_In b s1 -> f10 b = None) ->
+    f' b = Some (b', ofs) ->
+    ~sup_In b s1 -> sup_In b s1' ->
+    compose_meminj f10' f02' b = Some (b', ofs).
 Proof.
-  induction l1; intros; inv H.
-  - exploit H1. instantiate (1:= b1). eauto. intro. congruence.
-  - Abort.
+  induction s1'; intros; inv H.
+  - inv H4.
+  - destruct Mem.sup_dec in H6. eapply IHs1'; eauto.
+    destruct H4. congruence. auto.
+    destruct (eq_block a b). subst.
+    rewrite H2 in H6.
 
+    exploit update_properties. eauto.
+    intros. unfold meminj_add. destruct eq_block. subst. elim H. apply Mem.sup_incr_in1.
+    eapply H0. intro. apply H. apply Mem.sup_incr_in2. auto.
+    intros. unfold meminj_add. destruct eq_block. subst. elim H. left. auto.
+    eapply H1. intro. apply H. right. auto.
+    intros (INCR1 & INCR2 & ? & ?).
+    generalize (meminj_add_new f10 b (fresh_block s,0)). intro A.
+    generalize (meminj_add_new f02 (fresh_block s) (b',ofs)). intro B.
+    eapply compose_meminj_incr. eauto. eauto.
+    unfold compose_meminj. rewrite A, B. f_equal.
 
+    destruct (f' a) in H6.
+    eapply IHs1'; eauto.
+    intros. unfold meminj_add. destruct eq_block. subst. elim H. apply Mem.sup_incr_in1.
+    eapply H0. intro. apply H. apply Mem.sup_incr_in2. auto.
+    intros. unfold meminj_add. destruct eq_block. subst. elim H. left. auto.
+    apply H1. intro. apply H. right. auto. intro. destruct H; congruence.
+    destruct H4; congruence.
+    eapply IHs1'; eauto. destruct H4; congruence.
+Qed.
 
 Lemma inj_inj2:
   subcklr (inj @ inj) inj.
@@ -718,15 +719,14 @@ Proof.
   - intros w' m1' m2' H12 Hw12.
     destruct H12 as [f' m1' m2' Hm12].
     inversion Hw12 as [? ? ? ? ? ? Hf12' SEP12']. clear Hw12; subst.
-    set (a := update_meminj12 (Mem.support m1') f10 f02 f' (Mem.support m0)).
-    destruct a eqn: UPDATE. subst a.
-    rename m into f10'. rename m3 into f02'.
+    destruct (update_meminj12 (Mem.support m1) (Mem.support m1') f10 f02 f' (Mem.support m0)) as
+        [[f10' f02'] s'] eqn: UPDATE.
     exploit update_properties; eauto.
-    inv Hm02. eauto.
-    intros (INCR1 & INCR2 & SEP1 & SEP2).
+    inv Hm02. eauto. inv Hm10. eauto.
+    intros (INCR1 & INCR2 & SINC & SEP1 & SEP2).
     assert (exists m0',Mem.inject f10' m1' m0'
                   /\ Mem.inject f02' m0' m2'
-                  /\ Mem.sup_include (Mem.support m0) (Mem.support m0')).
+                  /\ Mem.support m0' = s').
     admit.
     destruct H1 as (m0' & INJ1 & INJ2 & SUP).
     exists ((injw f10' (Mem.support m1') (Mem.support m0')),(injw f02' (Mem.support m0') (Mem.support m2'))).
@@ -737,13 +737,21 @@ Proof.
       exploit SEP12'. unfold compose_meminj. rewrite H1. auto. rewrite A. reflexivity.
       intros [D E].
       split. auto. auto.
-      eauto. eauto.
+      eauto. rewrite SUP. eauto.
     + constructor. eauto.
       intros. exploit SEP2; eauto. intros [A B]. destruct B as (b0 & B & C).
       split. auto.
       exploit SEP12'. unfold compose_meminj. rewrite B. auto. rewrite C. reflexivity.
-      intros [D E]. auto. eauto. eauto.
-    + simpl. admit.
-Abort.
+      intros [D E]. auto. rewrite SUP. eauto. eauto.
+    + simpl. intro. intros.
+      destruct ((compose_meminj f10 f02) b) eqn: Hold. destruct p.
+      apply Hf12' in Hold as H00. rewrite H1 in H00. inv H00.
+      exploit compose_meminj_incr. apply INCR1. apply INCR2.
+      eauto. eauto.
+      exploit SEP12'; eauto. intros [A B].
+      eapply update_properties2; eauto. inv Hm02. eauto.
+      inv Hm10. eauto. inv Hm12. destruct (Mem.sup_dec b (Mem.support m1')).
+      auto. apply mi_freeblocks in n. congruence.
+Admitted.
 
 
